WIP

src/opt/ReorderFence.v
@@ -34,25 +34,25 @@ Inductive reorder_fence (or1 ow1:Ordering.t): forall (i2:Instr.t), Prop :=
     reorder_fence or1 ow1 (Instr.store l2 v2 o2)
 .
 
-Inductive sim_fence: forall (st_src:lang.(Language.state)) (lc_src:Local.t) (mem_k_src:Memory.t)
-                       (st_tgt:lang.(Language.state)) (lc_tgt:Local.t) (mem_k_tgt:Memory.t), Prop :=
+Inductive sim_fence: forall (st_src:lang.(Language.state)) (lc_src:Local.t) (sc_k_src:TimeMap.t) (mem_k_src:Memory.t)
+                       (st_tgt:lang.(Language.state)) (lc_tgt:Local.t) (sc_k_tgt:TimeMap.t) (mem_k_tgt:Memory.t), Prop :=
 | sim_fence_intro
     or1 ow1 i2
     rs lc1_src lc1_tgt lc2_src
     mem_k_src mem_k_tgt
     (REORDER: reorder_fence or1 ow1 i2)
-    (FENCE: Local.fence_step lc1_src mem_k_src or1 ow1 lc2_src)
+    (FENCE: Local.fence_step lc1_src sc_k_src mem_k_src or1 ow1 lc2_src)
     (LOCAL: sim_local lc2_src lc1_tgt):
     sim_fence
-      (State.mk rs [Stmt.instr i2; Stmt.instr (Instr.fence or1 ow1)]) lc1_src mem_k_src
-      (State.mk rs [Stmt.instr i2]) lc1_tgt mem_k_tgt
+      (State.mk rs [Stmt.instr i2; Stmt.instr (Instr.fence or1 ow1)]) lc1_src sc_k_src mem_k_src
+      (State.mk rs [Stmt.instr i2]) lc1_tgt sc_k_tgt mem_k_tgt
 .
 
 Lemma sim_fence_step
-      st1_src lc1_src mem_k_src
-      st1_tgt lc1_tgt mem_k_tgt
-      (SIM: sim_fence st1_src lc1_src mem_k_src
-                      st1_tgt lc1_tgt mem_k_tgt):
+      st1_src lc1_src sc_k_src mem_k_src
+      st1_tgt lc1_tgt sc_k_tgt mem_k_tgt
+      (SIM: sim_fence st1_src lc1_src sc_k_src mem_k_src
+                      st1_tgt lc1_tgt sc_k_tgt mem_k_tgt):
   forall mem1_src mem1_tgt
     (MEMORY: sim_memory mem1_src mem1_tgt)
     (FUTURE_SRC: Memory.future mem_k_src mem1_src)
@@ -92,7 +92,7 @@ Proof.
     + econs 2. econs 5; eauto. econs. econs.
     + eauto.
     + eauto.
-    + left. eapply paco7_mon; [apply sim_stmts_nil|]; ss.
+    + left. eapply paco9_mon; [apply sim_stmts_nil|]; ss.
 Qed.
 
 Lemma sim_fence_sim_thread:
@@ -111,6 +111,6 @@ Proof.
     apply MemInv.sem_bot_inv in PROMISES. rewrite PROMISES. auto.
   - ii. exploit sim_fence_step; eauto. i. des.
     + esplits; eauto.
-      left. eapply paco7_mon; eauto. ss.
+      left. eapply paco9_mon; eauto. ss.
     + esplits; eauto.
 Qed.
