src/opt/ReorderLoad.v
@@ -58,54 +58,60 @@ Inductive reorder_load r1 l1 o1: forall (i2:Instr.t), Prop :=
     reorder_load r1 l1 o1 (Instr.fence or2 ow2)
 .
 
-Inductive sim_load: forall (st_src:lang.(Language.state)) (lc_src:Local.t) (mem_k_src:Memory.t)
-                      (st_tgt:lang.(Language.state)) (lc_tgt:Local.t) (mem_k_tgt:Memory.t), Prop :=
+Inductive sim_load: forall (st_src:lang.(Language.state)) (lc_src:Local.t) (sc_k_src:TimeMap.t) (mem_k_src:Memory.t)
+                      (st_tgt:lang.(Language.state)) (lc_tgt:Local.t) (sc_k_tgt:TimeMap.t) (mem_k_tgt:Memory.t), Prop :=
 | sim_load_intro
     r1 l1 ts1 v1 released1 o1 i2
     rs lc1_src lc1_tgt lc2_src
+    sc_k_src sc_k_tgt
     mem_k_src mem_k_tgt
     (REORDER: reorder_load r1 l1 o1 i2)
     (READ: Local.read_step lc1_src mem_k_src l1 ts1 v1 released1 o1 lc2_src)
     (LOCAL: sim_local lc2_src lc1_tgt):
     sim_load
-      (State.mk rs [Stmt.instr i2; Stmt.instr (Instr.load r1 l1 o1)]) lc1_src mem_k_src
-      (State.mk (RegFun.add r1 v1 rs) [Stmt.instr i2]) lc1_tgt mem_k_tgt
+      (State.mk rs [Stmt.instr i2; Stmt.instr (Instr.load r1 l1 o1)]) lc1_src sc_k_src mem_k_src
+      (State.mk (RegFun.add r1 v1 rs) [Stmt.instr i2]) lc1_tgt sc_k_tgt mem_k_tgt
 .
 
 Lemma sim_load_step
-      st1_src lc1_src mem_k_src
-      st1_tgt lc1_tgt mem_k_tgt
-      (SIM: sim_load st1_src lc1_src mem_k_src
-                     st1_tgt lc1_tgt mem_k_tgt):
-  forall mem1_src mem1_tgt
-    (MEMORY: sim_memory mem1_src mem1_tgt)
-    (FUTURE_SRC: Memory.future mem_k_src mem1_src)
-    (FUTURE_TGT: Memory.future mem_k_tgt mem1_tgt)
+      st1_src lc1_src sc_k_src mem_k_src
+      st1_tgt lc1_tgt sc_k_tgt mem_k_tgt
+      (SIM: sim_load st1_src lc1_src sc_k_src mem_k_src
+                     st1_tgt lc1_tgt sc_k_tgt mem_k_tgt):
+  forall sc1_src sc1_tgt mem1_src mem1_tgt
+    (SC: TimeMap.le sc1_src sc1_tgt)
+    (MEMORY: Memory.sim mem1_tgt mem1_src)
+    (SC_FUTURE_SRC: TimeMap.le sc_k_src sc1_src)
+    (SC_FUTURE_TGT: TimeMap.le sc_k_tgt sc1_tgt)
+    (MEM_FUTURE_SRC: Memory.future mem_k_src mem1_src)
+    (MEM_FUTURE_TGT: Memory.future mem_k_tgt mem1_tgt)
     (WF_SRC: Local.wf lc1_src mem1_src)
     (WF_TGT: Local.wf lc1_tgt mem1_tgt)
+    (SC_SRC: Memory.closed_timemap sc1_src mem1_src)
+    (SC_TGT: Memory.closed_timemap sc1_tgt mem1_tgt)
     (MEM_SRC: Memory.closed mem1_src)
     (MEM_TGT: Memory.closed mem1_tgt),
-    _sim_thread_step lang lang ((sim_thread (sim_terminal eq)) \6/ sim_load)
-                     st1_src lc1_src mem1_src
-                     st1_tgt lc1_tgt mem1_tgt.
+    _sim_thread_step lang lang ((sim_thread (sim_terminal eq)) \8/ sim_load)
+                     st1_src lc1_src sc1_src mem1_src
+                     st1_tgt lc1_tgt sc1_tgt mem1_tgt.
 Proof.
   inv SIM. ii.
-  exploit Local.future_read_step; try apply READ; eauto. i.
-  inv STEP_TGT; inv STEP; try (inv STATE; inv INSTR; inv REORDER); ss.
+  exploit future_read_step; try apply READ; eauto. i. des.
+  inv STEP_TGT; inv STEP0; try (inv STATE; inv INSTR; inv REORDER); ss.
   - (* promise *)
-    exploit sim_local_promise; eauto.
+    exploit sim_local_promise; (try by etrans; eauto); eauto.
     { eapply Local.read_step_future; eauto. }
     i. des.
     exploit reorder_read_promise; try apply x0; try apply STEP_SRC; eauto. i. des.
-    esplits; eauto.
-    + econs. econs 1; eauto.
+    esplits; try apply SC; eauto.
+    + econs. econs. eauto.
     + eauto.
-    + right. econs; eauto.
+    + right. econs; eauto. etrans; eauto.
   - (* load *)
-    exploit sim_local_read; eauto.
+    exploit sim_local_read; (try by etrans; eauto); eauto.
     { eapply Local.read_step_future; eauto. }
     i. des.
-    exploit reorder_read_read; try apply x0; try apply STEP_SRC; eauto. i. des.
+    exploit reorder_read_read; try apply STEP; try apply STEP_SRC; eauto. i. des.
     esplits.
     + econs 2; [|econs 1]. econs.
       * econs 2. econs 2; eauto. econs. econs.
@@ -113,15 +119,19 @@ Proof.
     + econs 2. econs 2; eauto. econs. econs.
     + eauto.
     + eauto.
-    + left. eapply paco7_mon; [apply sim_stmts_nil|]; ss.
+    + eauto.
+    + left. eapply paco9_mon; [apply sim_stmts_nil|]; ss.
       apply RegFun.add_add. ii. subst. eapply REGS.
       * apply RegSet.singleton_spec. eauto.
       * apply RegSet.singleton_spec. eauto.
+      * etrans; eauto.
   - (* store *)
-    exploit sim_local_write; eauto.
+    exploit sim_local_write; try apply SC; try apply LOCAL1; (try by etrans; eauto); eauto.
+    { refl. }
+    { apply Capability.bot_wf. }
     { eapply Local.read_step_future; eauto. }
     i. des.
-    exploit reorder_read_write; try apply x0; try apply STEP_SRC; eauto. i. des.
+    exploit reorder_read_write; try apply STEP; try apply STEP_SRC; eauto. i. des.
     esplits.
     + econs 2; [|econs 1]. econs.
       * econs 2. econs 3; eauto. econs.
@@ -132,18 +142,20 @@ Proof.
     + econs 2. econs 2; eauto. econs. econs.
     + eauto.
     + eauto.
-    + left. eapply paco7_mon; [apply sim_stmts_nil|]; ss.
+    + eauto.
+    + left. eapply paco9_mon; [apply sim_stmts_nil|]; ss. etrans; eauto.
   - (* update *)
-    exploit sim_local_read; eauto.
+    exploit sim_local_read; (try by etrans; eauto); eauto.
     { eapply Local.read_step_future; eauto. }
     i. des.
-    exploit sim_local_write; eauto.
+    exploit sim_local_write; try apply SC; try apply LOCAL1; (try by etrans; eauto); eauto.
+    { admit. }
     { eapply Local.read_step_future; eauto.
       eapply Local.read_step_future; eauto.
     }
     { eapply Local.read_step_future; eauto. }
     i. des.
-    exploit reorder_read_read; try apply x0; try apply STEP_SRC; eauto. i. des.
+    exploit reorder_read_read; try apply STEP; try apply STEP_SRC; eauto. i. des.
     exploit reorder_read_write; try apply STEP2; try apply LOCAL2; eauto.
     { eapply Local.read_step_future; eauto. }
     i. des.
@@ -158,7 +170,7 @@ Proof.
     + econs 2. econs 2; eauto. econs. econs.
     + eauto.
     + eauto.
-    + left. eapply paco7_mon; [apply sim_stmts_nil|]; ss.
+    + left. eapply paco9_mon; [apply sim_stmts_nil|]; ss.
       apply RegFun.add_add. ii. subst. eapply REGS.
       * apply RegSet.singleton_spec. eauto.
       * apply RegSet.add_spec. eauto.
@@ -174,7 +186,7 @@ Proof.
     + econs 2. econs 2; eauto. econs. econs.
     + eauto.
     + eauto.
-    + left. eapply paco7_mon; [apply sim_stmts_nil|]; ss.
+    + left. eapply paco9_mon; [apply sim_stmts_nil|]; ss.
 Qed.
 
 Lemma sim_load_sim_thread:
@@ -193,6 +205,6 @@ Proof.
     apply MemInv.sem_bot_inv in PROMISES. rewrite PROMISES. auto.
   - ii. exploit sim_load_step; eauto. i. des.
     + esplits; eauto.
-      left. eapply paco7_mon; eauto. ss.
+      left. eapply paco9_mon; eauto. ss.
     + esplits; eauto.
 Qed.
