src/opt/ReorderStore.v
@@ -50,25 +50,25 @@ Inductive reorder_store l1 v1 o1: forall (i2:Instr.t), Prop :=
     reorder_store l1 v1 o1 (Instr.update r2 l2 rmw2 or2 ow2)
 .
 
-Inductive sim_store: forall (st_src:lang.(Language.state)) (lc_src:Local.t) (mem_k_src:Memory.t)
-                       (st_tgt:lang.(Language.state)) (lc_tgt:Local.t) (mem_k_tgt:Memory.t), Prop :=
+Inductive sim_store: forall (st_src:lang.(Language.state)) (lc_src:Local.t) (sc_k_src:TimeMap.t) (mem_k_src:Memory.t)
+                       (st_tgt:lang.(Language.state)) (lc_tgt:Local.t) (sc_k_tgt:TimeMap.t) (mem_k_tgt:Memory.t), Prop :=
 | sim_store_intro
     l1 f1 t1 v1 released1 o1 i2
     rs lc1_src lc1_tgt lc2_src
     mem_k_src mem_k_tgt
     (REORDER: reorder_store l1 v1 o1 i2)
-    (FULFILL: Local.fulfill_step lc1_src mem_k_src l1 f1 t1 (RegFile.eval_value rs v1) released1 released1 o1 lc2_src)
+    (FULFILL: Local.fulfill_step lc1_src sc_k_src mem_k_src l1 f1 t1 (RegFile.eval_value rs v1) released1 released1 o1 lc2_src)
     (LOCAL: sim_local lc2_src lc1_tgt):
     sim_store
-      (State.mk rs [Stmt.instr i2; Stmt.instr (Instr.store l1 v1 o1)]) lc1_src mem_k_src
-      (State.mk rs [Stmt.instr i2]) lc1_tgt mem_k_tgt
+      (State.mk rs [Stmt.instr i2; Stmt.instr (Instr.store l1 v1 o1)]) lc1_src sc_k_src mem_k_src
+      (State.mk rs [Stmt.instr i2]) lc1_tgt sc_k_tgt mem_k_tgt
 .
 
 Lemma sim_store_step
-      st1_src lc1_src mem_k_src
-      st1_tgt lc1_tgt mem_k_tgt
-      (SIM: sim_store st1_src lc1_src mem_k_src
-                      st1_tgt lc1_tgt mem_k_tgt):
+      st1_src lc1_src sc_k_src mem_k_src
+      st1_tgt lc1_tgt sc_k_tgt mem_k_tgt
+      (SIM: sim_store st1_src lc1_src sc_k_src mem_k_src
+                      st1_tgt lc1_tgt sc_k_tgt mem_k_tgt):
   forall mem1_src mem1_tgt
     (MEMORY: sim_memory mem1_src mem1_tgt)
     (FUTURE_SRC: Memory.future mem_k_src mem1_src)
@@ -109,7 +109,7 @@ Proof.
         { i. destruct o1; inv ORD1; inv H. }
     + eauto.
     + eauto.
-    + left. eapply paco7_mon; [apply sim_stmts_nil|]; ss.
+    + left. eapply paco9_mon; [apply sim_stmts_nil|]; ss.
   - (* store *)
     exploit sim_local_write; eauto.
     { eapply Local.fulfill_step_future; eauto. }
@@ -126,7 +126,7 @@ Proof.
         i. destruct o1; inv ORD1; inv H.
     + eauto.
     + eauto.
-    + left. eapply paco7_mon; [apply sim_stmts_nil|]; ss.
+    + left. eapply paco9_mon; [apply sim_stmts_nil|]; ss.
   - (* update *)
     exploit sim_local_read; eauto.
     { eapply Local.fulfill_step_future; eauto. }
@@ -153,7 +153,7 @@ Proof.
         { i. destruct o1; inv ORD1; inv H. }
     + eauto.
     + eauto.
-    + left. eapply paco7_mon; [apply sim_stmts_nil|]; ss.
+    + left. eapply paco9_mon; [apply sim_stmts_nil|]; ss.
 Qed.
 
 Lemma sim_store_sim_thread:
@@ -185,6 +185,6 @@ Proof.
     + inv SIM. inv STEP; inv STATE.
   - ii. exploit sim_store_step; eauto. i. des.
     + esplits; eauto.
-      left. eapply paco7_mon; eauto. ss.
+      left. eapply paco9_mon; eauto. ss.
     + esplits; eauto.
 Qed.
